\begin{solution}
The time that it takes the ball released at the surface to reach the bottom of the pool is

$$a = g\bigg(\frac{\rho_b - \rho_p}{\rho_b}\bigg) = rg$$

$$t = \sqrt{\frac{2d}{rg}}$$

The time that it takes the ball released above the surface is

$$t_1 = \sqrt{\frac{2h}{g}}$$

$$v_1 = at_1 = \sqrt{2gh}$$

$$v_2 = \sqrt{v_1^2 + 2ad} = \sqrt{2gh + 2rgd}$$

$$t_2 = \frac{v_2 - v_1}{a} = \frac{\sqrt{2gh + 2rgd} - \sqrt{2gh}}{rg}$$

The condition $t_1 + t_2 = t$ must be satisfied

$$\sqrt{\frac{2d}{rg}} = \sqrt{\frac{2h}{g}} + \frac{\sqrt{2gh + 2rgd} - \sqrt{2gh}}{rg}\longrightarrow\frac{\sqrt{2rd}}{r\sqrt{g}} = \frac{r\sqrt{2h} + \sqrt{2h + 2rd} - \sqrt{2h}}{r\sqrt{g}}$$

$$\sqrt{2rd} - (r-1)\sqrt{2h} = \sqrt{2h + 2rd}\longrightarrow 2rd - 4(r-1)\sqrt{rdh} + 2h(r-1)^2 = 2h + 2rd$$

$$h(r-1)^2 - 2(r-1)\sqrt{rdh} = h\longrightarrow 2(r-1)\sqrt{rdh} = h(r-1)^2 - h$$

$$\sqrt{d} = \frac{h(r-1)}{2\sqrt{rh}} - \frac{h}{2\sqrt{rh}(r-1)}\longrightarrow d = \frac{h(r-1)^2}{4r} - \frac{h}{2r} + \frac{h}{4r(r-1)^2}$$

$$d = \frac{(r-1)^4-2(r-1)^2 + 1}{4r(r-1)^2} h$$

$$d = \frac{r(r-2)^2}{4(r-1)^2}h = \frac{r^3 - 4r^2 + 4r}{4r^2-8r+4}h$$

The answer is thus $1-4+4+4-8+4=\boxed{1}$.
\end{solution}